Meta: restructure Meta
- Add UnanchoredEngine. Also prove that every AnchoredEngine is Unanchored when just running with a lazy_prefix
- Extract literal opts

Engine/Meta/EngineSpec.v
@@ -14,15 +14,16 @@ From Warblre Require Import Base RegExpRecord.
 
 
 Section Engines.
-  Context {VMS: VMSeen}.
   Context {params: LindenParameters}.
   Context (rer: RegExpRecord).
 
 (* interface of an anchored, executable engine *)
+(* an anchored engine finds matches exactly at the beginning of the input *)
 Class AnchoredEngine := {
   exec: regex -> input -> option leaf;
 
   (* asserts the supported subset of regexes *)
+  (* FIXME: these will need a decidable version for the Meta engine *)
   supported_regex: regex -> Prop;
 
   (* the execution follows the backtracking tree semantics *)
@@ -32,9 +33,50 @@ Class AnchoredEngine := {
     (first_leaf tree inp = ol <-> exec r inp = ol)
 }.
 
+Definition dot_star : regex :=
+  Quantified false 0 NoI.Inf (Regex.Character CdAll).
+Definition lazy_prefix (r:regex) : regex :=
+  Sequence dot_star r.
+
+(* interface of an unanchored, executable engine *)
+(* an unanchored engine finds matches anywhere in the input *)
+Class UnanchoredEngine := {
+  un_exec: regex -> input -> option leaf;
+
+  (* asserts the supported subset of regexes *)
+  un_supported_regex: regex -> Prop;
+
+  (* the execution follows the backtracking tree semantics *)
+  un_exec_correct: forall r inp tree ol,
+    un_supported_regex r ->
+    is_tree rer [Areg (lazy_prefix r)] inp Groups.GroupMap.empty forward tree ->
+    (first_leaf tree inp = ol <-> un_exec r inp = ol)
+}.
+End Engines.
+
+Section Instances.
+  Context {VMS: VMSeen}.
+  Context {params: LindenParameters}.
+  Context (rer: RegExpRecord).
+
+(* predicate stating that if we support a regex then we support its lazy prefix *)
+Definition lazy_prefix_supported {engine:AnchoredEngine rer} : Prop :=
+  forall r, supported_regex rer r -> supported_regex rer (lazy_prefix r).
+
+(* We show that any anchored engine can be turned into an unanchored engine by just *)
+(* executing the anchored engine with a lazy prefix *)
+#[refine]
+Instance UnanchorEngine {engine:AnchoredEngine rer} (lazy_prefix_supp: lazy_prefix_supported): UnanchoredEngine rer := {
+  un_exec r inp := exec rer (lazy_prefix r) inp;
+  un_supported_regex r := supported_regex rer r;
+}.
+  (* un_exec_correct *)
+  eauto using exec_correct.
+Qed.
+
 (* we show that the PikeVM fits the scheme of an anchored engine *)
 #[refine]
-Instance PikeVMAnchoredEngine: AnchoredEngine := {
+Instance PikeVMAnchoredEngine: AnchoredEngine rer := {
   exec r inp := match pike_vm_match rer r inp with
                 | OutOfFuel => None
                 | Finished res => res
@@ -51,4 +93,5 @@ Instance PikeVMAnchoredEngine: AnchoredEngine := {
   - intros <-.
     symmetry. eauto using pike_vm_match_correct, pike_vm_correct.
 Qed.
-End Engines.
+
+End Instances.
