Engine/Meta/MetaLiterals.v
@@ -1,0 +1,197 @@
+(** * Meta literals *)
+
+(* Different optimizations related to doing literal-based searches and acceleration. *)
+
+Require Import List.
+Import ListNotations.
+
+From Linden Require Import Regex Chars Semantics Tree.
+From Linden Require Import FunctionalUtils.
+From Linden Require Import Parameters LWParameters.
+From Linden Require Import StrictSuffix Prefix.
+From Linden Require Import EngineSpec.
+From Warblre Require Import Base RegExpRecord.
+
+
+Section MetaLiterals.
+  Context {params: LindenParameters}.
+  Context (rer: RegExpRecord).
+
+(* tries to perform a search using only the literal from the regex *)
+(* On success, returns the leaf. On failure, returns the literal. *)
+Definition try_lit_search {strs:StrSearch} (r:regex) (inp:input) : (option leaf) + literal :=
+  let lit := extract_literal rer r in
+  if lit == Impossible then inl None else
+		(* LATER: do a different search when we have Exact *)
+		inr lit.
+
+
+(* if the try_lit_search returned a leaf, it is the first_leaf *)
+Theorem try_lit_search_correct {strs:StrSearch}:
+	forall r inp tree ol,
+		is_tree rer [Areg (lazy_prefix r)] inp Groups.GroupMap.empty forward tree ->
+		try_lit_search r inp = inl ol ->
+		first_leaf tree inp = ol.
+Proof.
+	unfold try_lit_search.
+	intros r inp tree ol Htree Htry.
+	wt_eq.
+	- injection Htry as <-.
+		assert (extract_literal rer (lazy_prefix r) = Impossible). {
+			assert (RegExpRecord.ignoreCase rer = false). {
+				unfold extract_literal in Heq.
+				destruct (RegExpRecord.ignoreCase rer) eqn:Hic; [|reflexivity].
+				(* simpl in Heq. FIXME: why does Heq not reduce?? *)
+				admit.
+			}
+			simpl. now rewrite H, Heq.
+		}
+		eapply extract_literal_impossible; eauto.
+	- discriminate.
+Admitted.
+
+
+(** * Bruteforce search *)
+(* We define a search routine which attempts to run an anchored engine at each position *)
+(* returning the earliest result. We then prove that a prefix accelerated version is equivalent. *)
+
+(* for each input position we run the anchored engine and return the earliest match *)
+Fixpoint search_from {engine:AnchoredEngine rer} (r: regex) (next: string) (prev: string) : option leaf :=
+  match (exec rer r (Input next prev)) with
+  | Some leaf => Some leaf
+  | None => match next with
+            | [] => None
+            | c::t => search_from r t (c::prev)
+            end
+  end.
+
+Definition search_from_input {engine:AnchoredEngine rer} (r:regex) (inp:input) : option leaf :=
+  search_from r (next_str inp) (pref_str inp).
+
+
+(* same as search_from_input but skips input positions that do not match the prefix *)
+(* TODO: make it skip multiple times *)
+Definition search_from_input_acc {strs:StrSearch} {engine:AnchoredEngine rer} (r:regex) (inp:input) (lit:literal) : option leaf :=
+  let p := prefix lit in
+  (* we skip the initial input that does not match the prefix *)
+  match (input_search p inp) with
+  | None => None (* if prefix is not present anywhere, then we cannot match *)
+  | Some i => search_from r (next_str i) (pref_str i)
+  end.
+
+
+(* Fixpoint jump_try {strs:StrSearch} {engine:AnchoredEngine} (r:regex) (p:string) (next pref:string) : option leaf :=
+  (* we skip the initial input that does not match the prefix *)
+  match (input_search p (Input next pref)) with
+  | None => None (* if prefix is not present anywhere, then we cannot match *)
+  | Some (Input  =>
+      match (exec r (Input next pref)) with
+      | Some leaf => Some leaf
+      | None => match next with
+                | [] => None
+                | c::t => jump_try r p t (c::pref)
+                end
+      end
+  end. *)
+
+Lemma search_from_before_jump_eq {strs:StrSearch} {engine:AnchoredEngine rer}:
+  forall i r inp inp',
+    supported_regex rer r ->
+    input_search (prefix (extract_literal rer r)) inp = Some inp' ->
+    input_prefix i inp' forward ->
+    input_prefix inp i forward ->
+    search_from r (next_str i) (pref_str i) = search_from r (next_str inp') (pref_str inp').
+Proof.
+  intros i r inp inp' Hsubset Hsearch Hprefix Hlow.
+  remember forward as dir.
+  induction Hprefix; subst.
+  - reflexivity.
+  - pose proof H as Hadvance.
+    specialize (IHHprefix Hsearch).
+    unfold advance_input in H. destruct inp1 as [next1 pref1] eqn:Hinp1, next1 eqn:Hnext1; [easy|].
+    inversion H. rewrite <-H1 in IHHprefix.
+    assert (Hnone: exec rer r (Input (t :: s) pref1) = None). {
+      assert (Hbetween: input_between inp inp3 inp1). {
+        rewrite input_prefix_strict_suffix in Hprefix, Hlow.
+        split; destruct Hprefix, Hlow; subst; eauto using ss_next', ss_advance.
+      }
+      subst.
+      pose proof (is_tree_productivity rer [Areg r] (Input (t :: s) pref1) Groups.GroupMap.empty forward) as [tree Htree].
+      rewrite <-exec_correct; eauto.
+      eauto using input_search_no_earlier, extract_literal_prefix_contra.
+    }
+    simpl.
+    rewrite Hnone.
+    eauto using ip_prev'.
+Qed.
+
+Lemma input_search_exec_none {strs:StrSearch} {engine:AnchoredEngine rer}:
+  forall i r inp,
+    supported_regex rer r ->
+    input_search (prefix (extract_literal rer r)) inp = None ->
+    input_prefix inp i forward ->
+    exec rer r i = None.
+Proof.
+  intros i r inp Hsubset Hsearch Hlow.
+  rewrite input_prefix_strict_suffix in Hlow.
+  pose proof (is_tree_productivity rer [Areg r] i Groups.GroupMap.empty forward) as [tree Htree].
+  rewrite <-exec_correct; eauto.
+  eauto using input_search_not_found, extract_literal_prefix_contra.
+Qed.
+
+Lemma search_from_none_prefix {strs:StrSearch} {engine:AnchoredEngine rer}:
+  forall i r inp,
+    supported_regex rer r ->
+    input_search (prefix (extract_literal rer r)) inp = None ->
+    input_prefix inp i forward ->
+    search_from r (next_str i) (pref_str i) = None.
+Proof.
+  intros [next pref] r inp Hsubset Hsearch Hprefix.
+  generalize dependent pref.
+  induction next; intros pref Hprefix.
+  - simpl; erewrite input_search_exec_none; eauto using ip_eq.
+  - simpl in *.
+    erewrite IHnext. erewrite input_search_exec_none.
+    all: eauto using ip_prev'.
+Qed.
+
+Lemma input_search_exec_impossible {strs:StrSearch} {engine:AnchoredEngine rer}:
+  forall inp r,
+    supported_regex rer r ->
+    extract_literal rer r = Impossible ->
+    exec rer r inp = None.
+Proof.
+  intros inp r Hsubset Hextract.
+  pose proof (is_tree_productivity rer [Areg r] inp Groups.GroupMap.empty forward) as [tree Htree].
+  rewrite <-exec_correct; eauto.
+  eauto using extract_literal_impossible.
+Qed.
+
+Lemma search_from_impossible_prefix {strs:StrSearch} {engine:AnchoredEngine rer}:
+  forall inp r,
+    supported_regex rer r ->
+    extract_literal rer r = Impossible ->
+    search_from r (next_str inp) (pref_str inp) = None.
+Proof.
+  intros [next pref] r Hsubset Hextract.
+  generalize dependent pref.
+  induction next; intros pref; simpl; erewrite input_search_exec_impossible; eauto.
+Qed.
+
+Theorem builtin_exec_equiv {strs:StrSearch} {engine:AnchoredEngine rer}:
+  forall r inp,
+    supported_regex rer r ->
+    search_from_input r inp = search_from_input_acc r inp (extract_literal rer r).
+Proof.
+  intros r inp Hsubset.
+  unfold search_from_input, search_from_input_acc.
+  destruct input_search eqn:Hsearch.
+  - assert (input_prefix inp i forward). {
+      apply input_search_strict_suffix in Hsearch.
+      now rewrite <-input_prefix_strict_suffix in Hsearch.
+    }
+    eapply search_from_before_jump_eq; eauto using ip_eq.
+  - eapply search_from_none_prefix; eauto using ip_eq.
+Qed.
+
+End MetaLiterals.
